Basalt/Examples/NatList.lean
@@ -4,7 +4,7 @@ open RandomChoice
 
 namespace NatListExample
 
-def Nat.arbitrary : Gen Nat := do
+def Nat.arbitrary [Gen G] : G Nat := do
   pick
     (fun () => pure 0)
     (fun () => do
@@ -15,7 +15,7 @@ partial_fixpoint
 theorem Nat.arbitrary_support : n ∈ SPMF.support Nat.arbitrary := by
   induction n <;> rw [Nat.arbitrary] <;> simp [*]
 
-def List.arbitrary : Gen (List Nat) := do
+def List.arbitrary [Gen G] : G (List Nat) := do
   pick
     (fun () => pure [])
     (fun () => do
@@ -31,7 +31,7 @@ theorem List.arbitrary_support : SPMF.support List.arbitrary = Set.univ := by
   case _ => simp
   case _ x xs ih => simp [ih, Nat.arbitrary_support]
 
-def List.genSorted (m : Nat) : Gen (List Nat) := do
+def List.genSorted [Gen G] (m : Nat) : G (List Nat) := do
   pick
     (fun () => pure [])
     (fun () => do
@@ -41,7 +41,7 @@ def List.genSorted (m : Nat) : Gen (List Nat) := do
       return x :: xs)
 partial_fixpoint
 
-def List.diverge : Gen (List Nat) := do
+def List.diverge [Gen G] : G (List Nat) := do
   let x ← RandomChoice.choose 0 10 (by simp)
   let xs ← List.diverge
   return x :: xs
@@ -56,13 +56,13 @@ inductive ListF (α β : Type) where
   | nilStep : ListF α β
   | consStep : α → β → ListF α β
 
-def List.unfold (coalg : β → Gen (ListF α β)) (b : β) : Gen (List α) := do
+def List.unfold [Gen G] (coalg : β → G (ListF α β)) (b : β) : G (List α) := do
   match ← coalg b with
   | .nilStep => return []
   | .consStep x b' => return x :: (← List.unfold coalg b')
 partial_fixpoint
 
-def List.genSorted' (m : Nat) : Gen (List Nat) :=
+def List.genSorted' [Gen G] (m : Nat) : G (List Nat) :=
   List.unfold (fun m =>
     pick
       (fun () => pure .nilStep)
@@ -72,62 +72,8 @@ def List.genSorted' (m : Nat) : Gen (List Nat) :=
         return .consStep x x))
     m
 
-example : (List.genSorted m : SPMF _) = List.genSorted' m := by
-  apply SPMF.ext
-  intro xs
-  induction xs generalizing m with
-  | nil =>
-    rw [List.genSorted, List.genSorted', List.unfold]
-    rw [SPMF.bind_pick]
-    simp only [SPMF.pick_apply]
-    simp only [Bind.bind, Pure.pure, SPMF.pure, SPMF.bind, DFunLike.coe]
-    simp
-    nth_rewrite 1 [← add_zero (2⁻¹ : ENNReal)]
-    congr 1
-    symm
-    rw [mul_eq_zero]
-    right
-    rw [ENNReal.tsum_eq_zero]
-    intro a
-    cases a with
-    | nilStep => simp
-    | consStep x b' => simp
-  | cons x xs ih =>
-    rw [List.genSorted, List.genSorted', List.unfold]
-    rw [SPMF.bind_pick]
-    simp only [SPMF.pick_apply]
-    conv_rhs =>
-      enter [1, 2]
-      rw [pure_bind]
-    conv_rhs =>
-      enter [2, 2]
-      rw [bind_assoc]
-      enter [1, 2]
-      intro x
-      rw [pure_bind]
-      dsimp
-    dsimp [Pure.pure, SPMF.pure]
-    congr 1
-    refine congr_arg (HMul.hMul (1/2 : ENNReal)) ?_
-    simp only [Bind.bind, SPMF.bind, DFunLike.coe]
-    apply tsum_congr
-    intro delta
-    congr 1
-    dsimp [Bind.bind, SPMF.bind, SPMF.instFunLike]
-    apply tsum_congr
-    intro l
-    by_cases h : l = xs
-    · subst h
-      simp
-      split
-      · exact ih
-      · rfl
-    · have : x :: xs ≠ (m + delta) :: l := by
-        intro c; injection c with _ h'; subst h'; contradiction
-      simp [this]
-
 #guard_msgs(drop info) in
 #eval (for _ in [0:20] do
-  IO.println <| repr (← Gen.runIO List.arbitrary) : IO Unit)
+  IO.println <| repr (← List.arbitrary) : IO Unit)
 
 end NatListExample
