Basalt/Examples/Assert.lean
@@ -2,13 +2,13 @@ import Basalt
 
 open RandomChoice
 
-def assert (b : Bool) (f : b = true → Gen α) : Gen α :=
+def assert [Gen G] (b : Bool) (f : b = true → G α) : G α :=
   if h : b then f h else default
 
 example : (assert false (fun _ => pure 2) : SPMF _).mass = 0 := by
   simp [assert, default]
 
-def sampleUntilOne : Gen Unit := do
+def sampleUntilOne [Gen G] : G Unit := do
   if (← choose 0 1 (by simp)) == 1 then
     return ()
   else
