Basalt/Gen.lean
@@ -2,30 +2,27 @@ import Basalt.RandomChoice
 
 open Lean.Order
 
-/-!
-# Generator Representation
+class Gen (g : Type → Type) where
+  instInhabited : ∀ α, Inhabited (g α)
+  instMonad : Monad g
+  instRandomChoice : RandomChoice g
+  instCCPO : ∀ α, CCPO (g α)
+  instMonoBind : MonoBind g
 
-This file defines the top-level interface of PBT generators.
--/
+instance [m : Gen g] : ∀ α, Inhabited (g α) := m.instInhabited
+instance [m : Gen g] : Monad g := m.instMonad
+instance [m : Gen g] : RandomChoice g := m.instRandomChoice
+instance [m : Gen g] : ∀ α, CCPO (g α) := m.instCCPO
+instance [m : Gen g] : MonoBind g := m.instMonoBind
 
-/-- Our representation of generators abstracts over a number of type-classes, each of which provides
-  some important set of generator operations:
-- `Monad`: Generators compose monadically.
-- `RandomChoice`: Generators can express discrete random choices.
-- `Inhabited`: Generators can fail; there is a bottom value that represents non-termination and
-  other failures.
-- `CCPO` and `MonoBind`: Generators are partially-ordered and admit Knaster-Tarski fixed-points.
-  Generators that do not terminate structurally, or at all, are still expressable. (The monad's bind
-  operation should respect the partial order.)
-
-**NOTE**: I'm not sure this is actually right. This doesn't work well with higher-order generators,
-and it also makes `Gen` a `Type → Type 1`, which feels odd.
--/
-def Gen (α : Type) : Type 1 :=
-  ∀ {m : Type → Type}
-    [∀ α, Inhabited (m α)]
-    [Monad m]
-    [RandomChoice m]
-    [∀ α, CCPO (m α)]
-    [MonoBind m],
-    m α
+instance
+    [∀ α, Inhabited (g α)]
+    [Monad g]
+    [RandomChoice g]
+    [∀ α, CCPO (g α)]
+    [MonoBind g] : Gen g where
+  instInhabited := inferInstance
+  instMonad := inferInstance
+  instRandomChoice := inferInstance
+  instCCPO := inferInstance
+  instMonoBind := inferInstance
