Basalt/IO.lean
@@ -5,5 +5,3 @@ open RandomChoice
 
 instance : RandomChoice IO where
   choose lo hi _ := IO.rand lo hi
-
-def Gen.runIO (g : Gen α) : IO α := g
